tested autosubst2 on pi.sig

test/pi.sig
@@ -1,0 +1,13 @@
+-- Signature for System F
+
+-- the types
+chan : Type
+proc : Type
+
+-- the constructors for proc
+Nil : proc 
+Bang : proc -> proc 
+Res : (bind chan in proc) -> proc
+Par : proc -> proc -> proc 
+In : chan -> (bind chan in proc) -> proc
+Out : chan -> chan -> proc -> proc
