theories/CongLtLemma.v
@@ -6,7 +6,7 @@ Require Import Proc.
 
 
 
-Lemma lemma6: forall P Q P' a, 
+Lemma conga_resp_lt: forall P Q P' a, 
   lt P a P'-> conga P Q -> exists Q', lt Q a Q' /\ conga P' Q'.
 Proof.
 intros. 
@@ -197,6 +197,133 @@ exfalso. inversion H2.
 Qed.
 
 
+(*
+    -----------         ----------------------
+    P|0 conga P         (P|Q)|R  conga P|(Q|R)
+
+
+         ---------------
+         P|Q   conga Q|P
+
+*)
+
+(*
+Lemma cong_inv_conga: forall P Q, 
+  conga P Q -> 
+    exists P0, P0 cong 
+*)
+
+
+Hint Constructors lt cong conga: core. 
+
+Axiom skip: forall A, A.
+
+Lemma cong_resp_lt: forall P P' Q Q' a,  
+  cong P Q -> 
+   (lt P a P' -> exists Q0, lt Q a Q0 /\ cong P' Q0) /\
+   (lt Q a Q' -> exists P0, lt P a P0 /\ cong P0 Q').
+Proof. 
+intros. 
+generalize dependent P'.
+generalize dependent Q'. 
+induction H. 
+apply skip.
+apply skip.
+
+intros. split.
+intro. 
+assert(exists P0 : proc, lt Q a P0 /\ cong P0 Q').
+set (IHr:=IHcong P' P' ).
+destruct IHr.
+set (ex:= H2 H0).
+destruct ex.
+exists x. split.
+destruct H3.
+apply H3.
+destruct H3.
 
 
 
+
+
+
+(*
+Inductive lt: proc -> lab -> proc -> Prop :=
+| Lt_send: forall Q R P, lt (Send Q R P) (Lsend Q R) P 
+| Lt_rcv: forall Q P q, lt (Rcv Q P) (Lrcv Q q) (P.[q/])
+| Lt_parL: forall Q P P' a, lt P a P' -> lt (Par P Q) a (Par P' Q) 
+| Lt_parR: forall P Q Q' a, lt Q a Q' -> lt (Par P Q) a (Par P Q')
+| Lt_commL: forall P Q P' Q' q r, 
+    lt P (Lsend q r) P' -> lt Q (Lrcv q r) Q' -> lt (Par P Q) Ltau (Par P' Q')
+| Lt_commR: forall P Q P' Q' q r, 
+    lt P (Lrcv q r) P' -> lt Q (Lsend q r) Q' -> lt (Par P Q) Ltau (Par P' Q')
+.
+
+
+(*   (proc, |)  commutative monoid up to conga *)
+Inductive conga: proc -> proc -> Prop :=
+| Cga_parCom: forall P Q,     conga (Par P Q)  (Par Q P)
+| Cga_parAssoc: forall P Q R, conga (Par (Par P Q) R)    (Par P (Par Q R))
+| Cga_parNeut: forall P,      conga (Par P Zero) P
+.
+
+(*  cong = conga + equivrel + ctxrules *)
+Inductive cong: proc -> proc -> Prop :=
+| Cg_cga: forall P Q,     conga P Q -> cong P Q
+| Cg_refl: forall P,       cong P P
+| Cg_sym: forall P Q,     cong Q P -> cong P Q
+| Cg_trans: forall P Q R, cong P Q -> cong Q R -> cong P R
+| Cg_ctxParL: forall P P' Q, cong P P' -> cong (Par P Q) (Par P' Q)  
+| Cg_ctxParR: forall P Q Q', cong Q Q' -> cong (Par P Q) (Par P Q')
+| Cg_ctxSend: forall Q R P P', cong P P' -> cong (Send Q R P) (Send Q R P')
+| Cg_ctxRcv: forall Q P P', cong P P' -> cong (Rcv Q P) (Rcv Q P')
+.
+*)
+
+
+
+
+(*
+
+
+
+Lemma cong_resp_lt: forall P P' a, forall Q,  
+  cong P Q->  lt P a P' -> exists Q', lt Q a Q' /\ cong P' Q'.
+Proof. 
+intros.
+induction H. 
+(*===basecase conga===*)
+
+assert (exists Q0 : proc, lt Q a Q0 /\ conga P' Q0).
+apply (conga_resp_lt P Q P' a). apply H0. apply H.
+destruct H1.  
+exists x. destruct H1. split. apply H1. apply (Cg_cga P' x). apply H2.
+(*===basecase refl===*)
+
+exists P'. split. 
+apply H0. apply (Cg_refl P').
+(*===indcase sym===*)
+
+
+
+
+
+
+
+
+
+
+attempt with ind on P->a P'
+intros. generalize dependent Q.
+induction H. 
+
+(*===base case Lt_send===*)
+intros.   
+inversion H0. (*caseAn on Q!R.P cong Q0   *)
+ 
+exfalso. inversion H.
+
+exists P. split.
+apply (Lt_send Q R P). apply (Cg_refl P).
+
+*)
