test/output/picalc.v
@@ -1,0 +1,436 @@
+Require Import core unscoped.
+
+Require Import Setoid Morphisms Relation_Definitions.
+
+
+Module Core.
+
+Inductive chan : Type :=
+    var_chan : nat -> chan.
+
+Definition subst_chan (sigma_chan : nat -> chan) (s : chan) : chan :=
+  match s with
+  | var_chan s0 => sigma_chan s0
+  end.
+
+Lemma up_chan_chan (sigma : nat -> chan) : nat -> chan.
+Proof.
+exact (scons (var_chan var_zero)
+         (funcomp (subst_chan (funcomp (var_chan) shift)) sigma)).
+Defined.
+
+Lemma upId_chan_chan (sigma : nat -> chan)
+  (Eq : forall x, sigma x = var_chan x) :
+  forall x, up_chan_chan sigma x = var_chan x.
+Proof.
+exact (fun n =>
+       match n with
+       | S n' => ap (subst_chan (funcomp (var_chan) shift)) (Eq n')
+       | O => eq_refl
+       end).
+Qed.
+
+Definition idSubst_chan (sigma_chan : nat -> chan)
+  (Eq_chan : forall x, sigma_chan x = var_chan x) (s : chan) :
+  subst_chan sigma_chan s = s := match s with
+                                 | var_chan s0 => Eq_chan s0
+                                 end.
+
+Lemma upExt_chan_chan (sigma : nat -> chan) (tau : nat -> chan)
+  (Eq : forall x, sigma x = tau x) :
+  forall x, up_chan_chan sigma x = up_chan_chan tau x.
+Proof.
+exact (fun n =>
+       match n with
+       | S n' => ap (subst_chan (funcomp (var_chan) shift)) (Eq n')
+       | O => eq_refl
+       end).
+Qed.
+
+Definition ext_chan (sigma_chan : nat -> chan) (tau_chan : nat -> chan)
+  (Eq_chan : forall x, sigma_chan x = tau_chan x) (s : chan) :
+  subst_chan sigma_chan s = subst_chan tau_chan s :=
+  match s with
+  | var_chan s0 => Eq_chan s0
+  end.
+
+Definition compSubstSubst_chan (sigma_chan : nat -> chan)
+  (tau_chan : nat -> chan) (theta_chan : nat -> chan)
+  (Eq_chan : forall x,
+             funcomp (subst_chan tau_chan) sigma_chan x = theta_chan x)
+  (s : chan) :
+  subst_chan tau_chan (subst_chan sigma_chan s) = subst_chan theta_chan s :=
+  match s with
+  | var_chan s0 => Eq_chan s0
+  end.
+
+Lemma up_subst_subst_chan_chan (sigma : nat -> chan) (tau_chan : nat -> chan)
+  (theta : nat -> chan)
+  (Eq : forall x, funcomp (subst_chan tau_chan) sigma x = theta x) :
+  forall x,
+  funcomp (subst_chan (up_chan_chan tau_chan)) (up_chan_chan sigma) x =
+  up_chan_chan theta x.
+Proof.
+exact (fun n =>
+       match n with
+       | S n' =>
+           eq_trans
+             (compSubstSubst_chan (funcomp (var_chan) shift)
+                (up_chan_chan tau_chan)
+                (funcomp (up_chan_chan tau_chan) shift) (fun x => eq_refl)
+                (sigma n'))
+             (eq_trans
+                (eq_sym
+                   (compSubstSubst_chan tau_chan (funcomp (var_chan) shift)
+                      (funcomp (subst_chan (funcomp (var_chan) shift))
+                         tau_chan)
+                      (fun x => eq_refl) (sigma n')))
+                (ap (subst_chan (funcomp (var_chan) shift)) (Eq n')))
+       | O => eq_refl
+       end).
+Qed.
+
+Lemma substSubst_chan (sigma_chan : nat -> chan) (tau_chan : nat -> chan)
+  (s : chan) :
+  subst_chan tau_chan (subst_chan sigma_chan s) =
+  subst_chan (funcomp (subst_chan tau_chan) sigma_chan) s.
+Proof.
+exact (compSubstSubst_chan sigma_chan tau_chan _ (fun n => eq_refl) s).
+Qed.
+
+Lemma substSubst_chan_pointwise (sigma_chan : nat -> chan)
+  (tau_chan : nat -> chan) :
+  pointwise_relation _ eq
+    (funcomp (subst_chan tau_chan) (subst_chan sigma_chan))
+    (subst_chan (funcomp (subst_chan tau_chan) sigma_chan)).
+Proof.
+exact (fun s =>
+       compSubstSubst_chan sigma_chan tau_chan _ (fun n => eq_refl) s).
+Qed.
+
+Lemma instId'_chan (s : chan) : subst_chan (var_chan) s = s.
+Proof.
+exact (idSubst_chan (var_chan) (fun n => eq_refl) s).
+Qed.
+
+Lemma instId'_chan_pointwise :
+  pointwise_relation _ eq (subst_chan (var_chan)) id.
+Proof.
+exact (fun s => idSubst_chan (var_chan) (fun n => eq_refl) s).
+Qed.
+
+Lemma varL'_chan (sigma_chan : nat -> chan) (x : nat) :
+  subst_chan sigma_chan (var_chan x) = sigma_chan x.
+Proof.
+exact (eq_refl).
+Qed.
+
+Lemma varL'_chan_pointwise (sigma_chan : nat -> chan) :
+  pointwise_relation _ eq (funcomp (subst_chan sigma_chan) (var_chan))
+    sigma_chan.
+Proof.
+exact (fun x => eq_refl).
+Qed.
+
+Inductive proc : Type :=
+  | Nil : proc
+  | Bang : proc -> proc
+  | Res : proc -> proc
+  | Par : proc -> proc -> proc
+  | In : chan -> proc -> proc
+  | Out : chan -> chan -> proc -> proc.
+
+Lemma congr_Nil : Nil = Nil.
+Proof.
+exact (eq_refl).
+Qed.
+
+Lemma congr_Bang {s0 : proc} {t0 : proc} (H0 : s0 = t0) : Bang s0 = Bang t0.
+Proof.
+exact (eq_trans eq_refl (ap (fun x => Bang x) H0)).
+Qed.
+
+Lemma congr_Res {s0 : proc} {t0 : proc} (H0 : s0 = t0) : Res s0 = Res t0.
+Proof.
+exact (eq_trans eq_refl (ap (fun x => Res x) H0)).
+Qed.
+
+Lemma congr_Par {s0 : proc} {s1 : proc} {t0 : proc} {t1 : proc}
+  (H0 : s0 = t0) (H1 : s1 = t1) : Par s0 s1 = Par t0 t1.
+Proof.
+exact (eq_trans (eq_trans eq_refl (ap (fun x => Par x s1) H0))
+         (ap (fun x => Par t0 x) H1)).
+Qed.
+
+Lemma congr_In {s0 : chan} {s1 : proc} {t0 : chan} {t1 : proc} (H0 : s0 = t0)
+  (H1 : s1 = t1) : In s0 s1 = In t0 t1.
+Proof.
+exact (eq_trans (eq_trans eq_refl (ap (fun x => In x s1) H0))
+         (ap (fun x => In t0 x) H1)).
+Qed.
+
+Lemma congr_Out {s0 : chan} {s1 : chan} {s2 : proc} {t0 : chan} {t1 : chan}
+  {t2 : proc} (H0 : s0 = t0) (H1 : s1 = t1) (H2 : s2 = t2) :
+  Out s0 s1 s2 = Out t0 t1 t2.
+Proof.
+exact (eq_trans
+         (eq_trans (eq_trans eq_refl (ap (fun x => Out x s1 s2) H0))
+            (ap (fun x => Out t0 x s2) H1))
+         (ap (fun x => Out t0 t1 x) H2)).
+Qed.
+
+Fixpoint subst_proc (sigma_chan : nat -> chan) (s : proc) {struct s} : 
+proc :=
+  match s with
+  | Nil => Nil
+  | Bang s0 => Bang (subst_proc sigma_chan s0)
+  | Res s0 => Res (subst_proc (up_chan_chan sigma_chan) s0)
+  | Par s0 s1 => Par (subst_proc sigma_chan s0) (subst_proc sigma_chan s1)
+  | In s0 s1 =>
+      In (subst_chan sigma_chan s0) (subst_proc (up_chan_chan sigma_chan) s1)
+  | Out s0 s1 s2 =>
+      Out (subst_chan sigma_chan s0) (subst_chan sigma_chan s1)
+        (subst_proc sigma_chan s2)
+  end.
+
+Fixpoint idSubst_proc (sigma_chan : nat -> chan)
+(Eq_chan : forall x, sigma_chan x = var_chan x) (s : proc) {struct s} :
+subst_proc sigma_chan s = s :=
+  match s with
+  | Nil => congr_Nil
+  | Bang s0 => congr_Bang (idSubst_proc sigma_chan Eq_chan s0)
+  | Res s0 =>
+      congr_Res
+        (idSubst_proc (up_chan_chan sigma_chan) (upId_chan_chan _ Eq_chan) s0)
+  | Par s0 s1 =>
+      congr_Par (idSubst_proc sigma_chan Eq_chan s0)
+        (idSubst_proc sigma_chan Eq_chan s1)
+  | In s0 s1 =>
+      congr_In (idSubst_chan sigma_chan Eq_chan s0)
+        (idSubst_proc (up_chan_chan sigma_chan) (upId_chan_chan _ Eq_chan) s1)
+  | Out s0 s1 s2 =>
+      congr_Out (idSubst_chan sigma_chan Eq_chan s0)
+        (idSubst_chan sigma_chan Eq_chan s1)
+        (idSubst_proc sigma_chan Eq_chan s2)
+  end.
+
+Fixpoint ext_proc (sigma_chan : nat -> chan) (tau_chan : nat -> chan)
+(Eq_chan : forall x, sigma_chan x = tau_chan x) (s : proc) {struct s} :
+subst_proc sigma_chan s = subst_proc tau_chan s :=
+  match s with
+  | Nil => congr_Nil
+  | Bang s0 => congr_Bang (ext_proc sigma_chan tau_chan Eq_chan s0)
+  | Res s0 =>
+      congr_Res
+        (ext_proc (up_chan_chan sigma_chan) (up_chan_chan tau_chan)
+           (upExt_chan_chan _ _ Eq_chan) s0)
+  | Par s0 s1 =>
+      congr_Par (ext_proc sigma_chan tau_chan Eq_chan s0)
+        (ext_proc sigma_chan tau_chan Eq_chan s1)
+  | In s0 s1 =>
+      congr_In (ext_chan sigma_chan tau_chan Eq_chan s0)
+        (ext_proc (up_chan_chan sigma_chan) (up_chan_chan tau_chan)
+           (upExt_chan_chan _ _ Eq_chan) s1)
+  | Out s0 s1 s2 =>
+      congr_Out (ext_chan sigma_chan tau_chan Eq_chan s0)
+        (ext_chan sigma_chan tau_chan Eq_chan s1)
+        (ext_proc sigma_chan tau_chan Eq_chan s2)
+  end.
+
+Fixpoint compSubstSubst_proc (sigma_chan : nat -> chan)
+(tau_chan : nat -> chan) (theta_chan : nat -> chan)
+(Eq_chan : forall x,
+           funcomp (subst_chan tau_chan) sigma_chan x = theta_chan x)
+(s : proc) {struct s} :
+subst_proc tau_chan (subst_proc sigma_chan s) = subst_proc theta_chan s :=
+  match s with
+  | Nil => congr_Nil
+  | Bang s0 =>
+      congr_Bang
+        (compSubstSubst_proc sigma_chan tau_chan theta_chan Eq_chan s0)
+  | Res s0 =>
+      congr_Res
+        (compSubstSubst_proc (up_chan_chan sigma_chan)
+           (up_chan_chan tau_chan) (up_chan_chan theta_chan)
+           (up_subst_subst_chan_chan _ _ _ Eq_chan) s0)
+  | Par s0 s1 =>
+      congr_Par
+        (compSubstSubst_proc sigma_chan tau_chan theta_chan Eq_chan s0)
+        (compSubstSubst_proc sigma_chan tau_chan theta_chan Eq_chan s1)
+  | In s0 s1 =>
+      congr_In
+        (compSubstSubst_chan sigma_chan tau_chan theta_chan Eq_chan s0)
+        (compSubstSubst_proc (up_chan_chan sigma_chan)
+           (up_chan_chan tau_chan) (up_chan_chan theta_chan)
+           (up_subst_subst_chan_chan _ _ _ Eq_chan) s1)
+  | Out s0 s1 s2 =>
+      congr_Out
+        (compSubstSubst_chan sigma_chan tau_chan theta_chan Eq_chan s0)
+        (compSubstSubst_chan sigma_chan tau_chan theta_chan Eq_chan s1)
+        (compSubstSubst_proc sigma_chan tau_chan theta_chan Eq_chan s2)
+  end.
+
+Lemma substSubst_proc (sigma_chan : nat -> chan) (tau_chan : nat -> chan)
+  (s : proc) :
+  subst_proc tau_chan (subst_proc sigma_chan s) =
+  subst_proc (funcomp (subst_chan tau_chan) sigma_chan) s.
+Proof.
+exact (compSubstSubst_proc sigma_chan tau_chan _ (fun n => eq_refl) s).
+Qed.
+
+Lemma substSubst_proc_pointwise (sigma_chan : nat -> chan)
+  (tau_chan : nat -> chan) :
+  pointwise_relation _ eq
+    (funcomp (subst_proc tau_chan) (subst_proc sigma_chan))
+    (subst_proc (funcomp (subst_chan tau_chan) sigma_chan)).
+Proof.
+exact (fun s =>
+       compSubstSubst_proc sigma_chan tau_chan _ (fun n => eq_refl) s).
+Qed.
+
+Lemma instId'_proc (s : proc) : subst_proc (var_chan) s = s.
+Proof.
+exact (idSubst_proc (var_chan) (fun n => eq_refl) s).
+Qed.
+
+Lemma instId'_proc_pointwise :
+  pointwise_relation _ eq (subst_proc (var_chan)) id.
+Proof.
+exact (fun s => idSubst_proc (var_chan) (fun n => eq_refl) s).
+Qed.
+
+Class Up_proc X Y :=
+    up_proc : X -> Y.
+
+Class Up_chan X Y :=
+    up_chan : X -> Y.
+
+#[global] Instance Subst_proc : (Subst1 _ _ _) := @subst_proc.
+
+#[global] Instance Up_chan_chan : (Up_chan _ _) := @up_chan_chan.
+
+#[global] Instance Subst_chan : (Subst1 _ _ _) := @subst_chan.
+
+#[global]
+Instance VarInstance_chan : (Var _ _) := @var_chan.
+
+Notation "s [ sigma_chan ]" := (subst_proc sigma_chan s)
+( at level 7, left associativity, only printing)  : subst_scope.
+
+Notation "↑__proc" := up_proc (only printing)  : subst_scope.
+
+Notation "↑__chan" := up_chan_chan (only printing)  : subst_scope.
+
+Notation "s [ sigma_chan ]" := (subst_chan sigma_chan s)
+( at level 7, left associativity, only printing)  : subst_scope.
+
+Notation "↑__chan" := up_chan (only printing)  : subst_scope.
+
+Notation "'var'" := var_chan ( at level 1, only printing)  : subst_scope.
+
+Notation "x '__chan'" := (@ids _ _ VarInstance_chan x)
+( at level 5, format "x __chan", only printing)  : subst_scope.
+
+Notation "x '__chan'" := (var_chan x) ( at level 5, format "x __chan")  :
+subst_scope.
+
+#[global]
+Instance subst_proc_morphism :
+ (Proper (respectful (pointwise_relation _ eq) (respectful eq eq))
+    (@subst_proc)).
+Proof.
+exact (fun f_chan g_chan Eq_chan s t Eq_st =>
+       eq_ind s (fun t' => subst_proc f_chan s = subst_proc g_chan t')
+         (ext_proc f_chan g_chan Eq_chan s) t Eq_st).
+Qed.
+
+#[global]
+Instance subst_proc_morphism2 :
+ (Proper (respectful (pointwise_relation _ eq) (pointwise_relation _ eq))
+    (@subst_proc)).
+Proof.
+exact (fun f_chan g_chan Eq_chan s => ext_proc f_chan g_chan Eq_chan s).
+Qed.
+
+#[global]
+Instance subst_chan_morphism :
+ (Proper (respectful (pointwise_relation _ eq) (respectful eq eq))
+    (@subst_chan)).
+Proof.
+exact (fun f_chan g_chan Eq_chan s t Eq_st =>
+       eq_ind s (fun t' => subst_chan f_chan s = subst_chan g_chan t')
+         (ext_chan f_chan g_chan Eq_chan s) t Eq_st).
+Qed.
+
+#[global]
+Instance subst_chan_morphism2 :
+ (Proper (respectful (pointwise_relation _ eq) (pointwise_relation _ eq))
+    (@subst_chan)).
+Proof.
+exact (fun f_chan g_chan Eq_chan s => ext_chan f_chan g_chan Eq_chan s).
+Qed.
+
+Ltac auto_unfold := repeat
+                     unfold VarInstance_chan, Var, ids, Subst_chan, Subst1,
+                      subst1, Up_chan_chan, Up_chan, up_chan, Subst_proc,
+                      Subst1, subst1.
+
+Tactic Notation "auto_unfold" "in" "*" := repeat
+                                           unfold VarInstance_chan, Var, ids,
+                                            Subst_chan, Subst1, subst1,
+                                            Up_chan_chan, Up_chan, up_chan,
+                                            Subst_proc, Subst1, subst1 
+                                            in *.
+
+Ltac asimpl' := repeat (first
+                 [ progress setoid_rewrite substSubst_proc_pointwise
+                 | progress setoid_rewrite substSubst_proc
+                 | progress setoid_rewrite substSubst_chan_pointwise
+                 | progress setoid_rewrite substSubst_chan
+                 | progress setoid_rewrite instId'_proc_pointwise
+                 | progress setoid_rewrite instId'_proc
+                 | progress setoid_rewrite varL'_chan_pointwise
+                 | progress setoid_rewrite varL'_chan
+                 | progress setoid_rewrite instId'_chan_pointwise
+                 | progress setoid_rewrite instId'_chan
+                 | progress unfold up_chan_chan, up_ren
+                 | progress cbn[subst_proc subst_chan]
+                 | progress fsimpl ]).
+
+Ltac asimpl := check_no_evars;
+                repeat
+                 unfold VarInstance_chan, Var, ids, Subst_chan, Subst1,
+                  subst1, Up_chan_chan, Up_chan, up_chan, Subst_proc, Subst1,
+                  subst1 in *;
+                asimpl'; minimize.
+
+Tactic Notation "asimpl" "in" hyp(J) := revert J; asimpl; intros J.
+
+Tactic Notation "auto_case" := auto_case ltac:(asimpl; cbn; eauto).
+
+Ltac substify := auto_unfold.
+
+Ltac renamify := auto_unfold.
+
+End Core.
+
+Module Extra.
+
+Import Core.
+
+#[global] Hint Opaque subst_proc: rewrite.
+
+#[global] Hint Opaque subst_chan: rewrite.
+
+End Extra.
+
+Module interface.
+
+Export Core.
+
+Export Extra.
+
+End interface.
+
+Export interface.
+
